theories/Example.v
@@ -53,3 +53,18 @@ Ltac auto_star ::=
               solve [ math 
                     | auto_false_base ltac:(fun tt => intuition eauto) ] ].
 
+
+(* LATER: move to TLC *)
+
+Definition max (n m:int) : int := 
+  If n > m then n else m.
+
+Lemma max_nonpos : forall n,
+  n <= 0 ->
+  max 0 n = 0.
+Proof using. introv M. unfold max. case_if; math. Qed.
+
+Lemma max_nonneg : forall n,
+  n >= 0 ->
+  max 0 n = n.
+Proof using. introv M. unfold max. case_if; math. Qed.
